ulib/FStar.Int.fst
@@ -103,7 +103,7 @@ let ones_from_vec_lemma #n =
   to_vec_lemma_2 (from_vec (ones_vec #n)) (ones n)
 
 let nth_lemma #n a b =
-  assert(forall (i:nat{i < n}). index (to_vec #n a) i = index (to_vec #n b) i);
+  assert(forall (i:nat{i < n}). {:nopattern} index (to_vec #n a) i = index (to_vec #n b) i);
   to_vec_lemma_2 a b
 
 let zero_nth_lemma #n i = ()
