_compare/run_base.sh
@@ -1,0 +1,20 @@
+#!/bin/bash
+set -e
+BASE_FSTAR=/home/nswamy/clean/FStar-base/stage2/out/bin/fstar.exe
+SRC=ulib/
+CACHE_DIR=_compare/base/checked/
+OUTPUT_DIR=_compare/base/ml/
+CODEGEN=OCaml
+TAG=base
+
+mkdir -p $CACHE_DIR $OUTPUT_DIR
+
+env \
+  SRC=$SRC \
+  FSTAR_EXE=$BASE_FSTAR \
+  CACHE_DIR=$CACHE_DIR \
+  OUTPUT_DIR=$OUTPUT_DIR \
+  CODEGEN=$CODEGEN \
+  TAG=$TAG \
+  FSTAR_OPTIONS="--log_queries" \
+  make -skj$(nproc) -f mk/lib.mk verify 2>&1
