qipatterns.md
@@ -1,0 +1,62 @@
+We have a proposal for something you could work on.  Right now, when people write "forall" and "exists" in F*, they can write a Z3 pattern (trigger) using the "{:pattern ...}" syntax ( https://github.com/FStarLang/FStar/wiki/Quantifiers-and-patterns ).  However, if people don't write these patterns, then Z3 chooses the pattern, and Z3 does not have enough information to choose good patterns.  Dafny faced the same situation a few years ago, and Clement addressed this issue by extending Dafny to automatically choose good forall/exists triggers before sending queries to Z3.  You may be familiar with Dafny's trigger-generation code already; I was looking for commits related to it and I saw that you improved some of the code that Clement wrote:
+ 
+https://github.com/Microsoft/dafny/commit/5eb855972c191ed6323253329fc50ebd1683fdd6
+ 
+We'd like to have a similar automatic pattern generation for F* forall and exists.  It does not have to be as sophisticated as Dafny's, though, at least to start with.  For simplicity, I propose that (at least to start with), we not try to infer conjunctions of patterns {:pattern e1; ...; ek}.  I checked the haclstar repo, and:
+•	about 2% of all user-supplied patterns use conjunctions ";".
+•	about 20% of all user-supplied patterns use disjunctions "\/".
+F* ulib is a little higher (10% with ";" and 30% with "\/"), but I don't think inferring conjunctions ";" is essential to start with.
+ 
+Here's a simple proposal that would get us started.  Roughly, it's "find the smallest terms that contain all the quantifier variables".  In more detail:
+•	If a user writes {:pattern ...} on a forall/exists, then F* uses the user-supplied pattern (no automated generation).
+•	If a user writes {:nopattern} on a forall/exists, then F* generates no pattern and therefore lets Z3 choose the pattern.
+•	Otherwise, F* attempts to automatically generate patterns for the forall/exist.
+o	If the generation fails, then F* emits a warning asking the user to supply a {:pattern} or {:nopattern}, defaulting to the behavior of nopattern (i.e. letting Z3 choose the pattern).
+o	(Eventually, I'd like to emit an error in this case.)
+•	To automatically generate patterns for (forall (x1...xn). e) or (exists (x1...xn). e), F* searches inside e for a term t that contains all the variables x1...xn:
+o	For simplicity, the search need not look inside other binders, such as nested foralls, exists, let, or lambdas inside e.
+	(this could be improved, but it will prevent accidentally generating patterns that include out-of-scope variables)
+o	The term t should contain only function applications, constants, and variables.  It should contain at least one function application (i.e. it can't just be a variable by itself).  It should not contain:
+	any function with the "[@smt_theory_symbol]" attribute, like /\, ==, +, etc.
+	"let", foralls, exists, and lambdas
+o	F* should make t as small as possible while still covering x1...xn.  For example, it should choose f(x, y) instead of h(f(x, y)).
+o	If there are no such t, automatic generation fails.
+o	There may be more than one t.  In this case, F* would generate a disjunction of the terms {:pattern t1 \/ ... \/ tk}.
+To avoid breaking old code, F* would only try to infer patterns if the --ext auto_patterns flag is set on the command line.
+ 
+Examples:
+•	(forall x. f(x) == h(g(x)))
+o	generates {:pattern f(x) \/ g(x)}
+•	(forall x. h(f(x), g(x)))
+o	generates {:pattern f(x) \/ g(x)}
+•	(forall x. f(x) == f(x + 1) /\ g(x))
+o	generates {:pattern f(x) \/ g(x)}
+o	(this is actually bad because f(x) leads to a matching loop, but we can try to improve this later)
+•	(forall x y. h(f(x), g(y)))
+o	generates {:pattern h(f(x), g(y))}
+•	(forall x y. f(x) == f(y))
+o	fails, because this requires a conjunctive pattern {:pattern f(x); f(y)}
+•	(forall x. let y = x + 1 in f(x) == g(x, y))
+o	fails, because f(x) and g(x, y) are inside a let-binding
+ 
+In terms of implementation strategy, I would suggest adding it in TcTerm, in the
+case of Tm_app. 
+
+Note, the representation quantifiers like `forall x1 .. xn. e` in AST a nested
+application of 
+`Tm_app(Tm_fvar (forall), (fun x1 -> Tm_App(..., (fun xn -> e))))`, 
+and the pattern has to go on the innermost application, so that it applies to all the variables x1...xn. 
+
+So, to handle this, I would suggest adding some logic to the Tm_app case, which triggers in phase2 only:
+- it detects if the head symbol is a quantifier (forall or exists)
+- if so, it descends into the term, finding the innermost application of the quantifier, and then checking for the presence of a user-supplied pattern or nopattern. If neither is present, then it tries to generate a pattern as described above.
+- then it returns the elaborated term with the inferred pattern, which it passes as
+normal to the rest of the phase2 typechecking process. 
+
+All of this logic should be guarded under the --ext auto_patterns flag.
+
+Once you have it implemented, start enabling it in ulib files and benchmark carefully, first noting
+- if you find files that regress with the new pattern generation, make a careful note of it add :nopattern annotations to the relevant quantifiers in those files, and make a log
+of such changes
+
+
